coq/SoundSet.v
@@ -358,6 +358,60 @@ eauto.
 Qed.
 
 
+Lemma sound_iset_formation :
+  forall G a a' b b',
+    pseq G (deqtype a a')
+    -> pseq (cons (hyp_tm a) G) (deqtype b b')
+    -> pseq G (deqtype (iset a b) (iset a' b')).
+Proof.
+intros G a b c d.
+revert G.
+refine (seq_pseq 2 [hyp_emp] c [hyp_emp] d 2 [] _ [_] _ _ _); cbn.
+intros G Hclc Hcld Hseqab Hseqcd.
+rewrite -> seq_eqtype in Hseqab, Hseqcd |- *.
+intros i s s' Hs.
+so (seqctx_impl_closub _#4 (pwctx_impl_seqctx _#4 Hs)) as (Hcls & Hcls').
+so (Hseqab _#3 Hs) as (A & Hal & Har & Hbl & Hbr).
+assert (den A = ceiling (S i) (den A)) as HeqA.
+  {
+  so (basic_impl_iutruncate _#6 Hal) as Heq.
+  exact (f_equal den Heq).
+  }
+exploit (extract_functional_multi toppg i (den A) (subst (under 1 s) c) (subst (under 1 s') c) (subst (under 1 s) d) (subst (under 1 s') d)) as (C & Hcl & Hcr & Hdl & Hdr); eauto using subst_closub_under_permit.
+  {
+  intros j m p Hmp.
+  assert (pwctx j (dot m s) (dot p s') (cons (hyp_tm a) G)) as Hss.
+    {
+    assert (j <= i) as Hj.
+      {
+      rewrite -> HeqA in Hmp.
+      destruct Hmp.
+      omega.
+      }
+    apply pwctx_cons_tm_seq; eauto using pwctx_downward.
+      {
+      eapply seqhyp_tm_leq; eauto using interp_increase, toppg_max.
+      }
+
+      {
+      intros j' t t' Ht.
+      so (Hseqab _#3 Ht) as (R & Hl & Hr & _).
+      eauto.
+      }
+    }
+  so (Hseqcd _#3 Hss) as (R & Hcl & Hcr & Hdl & Hdr).
+  exists R.
+  simpsub.
+  auto.
+  }
+exists (iuiset stop A C).
+simpsub.
+do2 3 split; auto;
+apply interp_eval_refl;
+apply interp_iset; auto.
+Qed.
+
+
 Lemma sound_set_formation_univ :
   forall G lv a a' b b' mr ml,
     pseq G (deq a a' (univ lv))
@@ -409,6 +463,62 @@ exploit (sound_set_formation_main (Some lv) G a b c d mr ml) as H; auto.
   so (Hseqdc _#3 Hs) as (R & Hl & Hr & Hm & _).
   eauto.
   }
+Qed.
+
+
+Lemma sound_iset_formation_univ :
+  forall G lv a a' b b',
+    pseq G (deq a a' (univ lv))
+    -> pseq (cons (hyp_tm a) G) (deq b b' (univ (subst sh1 lv)))
+    -> pseq G (deq (iset a b) (iset a' b') (univ lv)).
+Proof.
+intros G lv a b c d.
+revert G.
+refine (seq_pseq 2 [hyp_emp] c [hyp_emp] d 2 [] _ [_] _ _ _); cbn.
+intros G Hclc Hcld Hseqab Hseqcd.
+rewrite -> seq_univ in Hseqab, Hseqcd |- *.
+intros i s s' Hs.
+so (seqctx_impl_closub _#4 (pwctx_impl_seqctx _#4 Hs)) as (Hcls & Hcls').
+so (Hseqab _#3 Hs) as (pg & A & Hlvl & Hlvr & Hal & Har & Hbl & Hbr).
+assert (den A = ceiling (S i) (den A)) as HeqA.
+  {
+  so (basic_impl_iutruncate _#6 Hal) as Heq.
+  exact (f_equal den Heq).
+  }
+exploit (extract_functional_multi pg i (den A) (subst (under 1 s) c) (subst (under 1 s') c) (subst (under 1 s) d) (subst (under 1 s') d)) as (C & Hcl & Hcr & Hdl & Hdr); eauto using subst_closub_under_permit.
+  {
+  intros j m p Hmp.
+  assert (pwctx j (dot m s) (dot p s') (cons (hyp_tm a) G)) as Hss.
+    {
+    assert (j <= i) as Hj.
+      {
+      rewrite -> HeqA in Hmp.
+      destruct Hmp.
+      omega.
+      }
+    apply pwctx_cons_tm_seq; eauto using pwctx_downward.
+      {
+      eapply seqhyp_tm_leq; eauto using interp_increase, toppg_max.
+      }
+
+      {
+      intros j' t t' Ht.
+      so (Hseqab _#3 Ht) as (pg' & R & _ & _ & Hl & Hr & _).
+      eauto.
+      }
+    }
+  so (Hseqcd _#3 Hss) as (pg' & R & Hlvl' & _ & Hcl & Hcr & Hdl & Hdr).
+  simpsubin Hlvl'.
+  so (pginterp_fun _#3 Hlvl Hlvl'); subst pg'.
+  exists R.
+  simpsub.
+  auto.
+  }
+exists pg, (iuiset stop A C).
+simpsub.
+do2 5 split; auto;
+apply interp_eval_refl;
+apply interp_iset; auto.
 Qed.
 
 
@@ -497,6 +607,91 @@ try (apply interp_eval_refl;
 Qed.
 
 
+Lemma sound_iset_intro :
+  forall G a b m n p,
+    pseq G (deq m n a)
+    -> pseq G (deq p p (subst1 m b))
+    -> pseq (hyp_tm a :: G) (deqtype b b)
+    -> pseq G (deq m n (iset a b)).
+Proof.
+intros G a b m n p.
+revert G.
+refine (seq_pseq 1 [hyp_emp] b 3 [] _ [] _ [_] _ _ _); cbn.
+intros G Hclb Hseqmn Hseqp Hseqb.
+rewrite -> seq_eqtype in Hseqb.
+rewrite -> seq_deq in Hseqmn, Hseqp |- *.
+intros i s s' Hs.
+so (pwctx_impl_closub _#4 Hs) as (Hcls & Hcls').
+so (Hseqmn _#3 Hs) as (A & Hal & Har & Hm & Hn & Hmn).
+assert (den A = ceiling (S i) (den A)) as HeqA.
+  {
+  so (basic_impl_iutruncate _#6 Hal) as Heq.
+  exact (f_equal den Heq).
+  }
+exploit (extract_functional toppg i (den A) (subst (under 1 s) b) (subst (under 1 s') b)) as (B & Hbl & Hbr); eauto using subst_closub_under_permit.
+  {
+  intros j r t Hrt.
+  assert (pwctx j (dot r s) (dot t s') (cons (hyp_tm a) G)) as Hss.
+    {
+    assert (j <= i) as Hj.
+      {
+      rewrite -> HeqA in Hrt.
+      destruct Hrt.
+      omega.
+      }
+    apply pwctx_cons_tm_seq; eauto using pwctx_downward.
+      {
+      eapply seqhyp_tm_leq; eauto using interp_increase, toppg_max.
+      }
+
+      {
+      intros j' u u' Hu.
+      so (Hseqmn _#3 Hu) as (R & Hl & Hr & _).
+      eauto.
+      }
+    }
+  so (Hseqb _#3 Hss) as (R & Hbl & Hbr & _).
+  exists R.
+  simpsub.
+  auto.
+  }
+so (Hseqp _#3 Hs) as (Bm & Hbml & _ & Hp & _).
+simpsubin Hbml.
+invert Hbl.
+intros _ _ Hact.
+so (Hact _#3 (le_refl _) Hm) as H.
+simpsubin H.
+so (basic_fun _#7 H Hbml); subst Bm; clear H Hbml.
+exists (iuiset stop A B).
+simpsub.
+do2 4 split;
+try (apply interp_eval_refl;
+     apply interp_iset; auto).
+  {
+  cbn.
+  exists (subst s p), (subst s' p), Hm.
+  auto.
+  }
+
+  {
+  cbn.
+  exists (subst s p), (subst s' p), Hn.
+  force_exact Hp.
+  do 3 f_equal.
+  apply urelspinj_equal; auto.
+  }
+
+
+  {
+  cbn.
+  exists (subst s p), (subst s' p), Hmn.
+  force_exact Hp.
+  do 3 f_equal.
+  apply urelspinj_equal; auto.
+  }
+Qed.
+
+
 Lemma sound_set_elim1 :
   forall G a b m n,
     pseq G (deq m n (set a b))
@@ -519,6 +714,55 @@ so (eqtrans Heq1 (eqsymm Heq2)) as Heq.
 clear Heq2.
 subst R.
 so (iuset_inj _#5 Heq); subst A'.
+exists A.
+do2 4 split; auto.
+  {
+  cbn in Hm.
+  decompose Hm.
+  intros _ _ H _.
+  auto.
+  }
+
+  {
+  cbn in Hn.
+  decompose Hn.
+  intros _ _ H _.
+  auto.
+  }
+
+  {
+  cbn in Hmn.
+  decompose Hmn.
+  intros _ _ H _.
+  auto.
+  }
+Qed.
+
+
+Lemma sound_iset_elim1 :
+  forall G a b m n,
+    pseq G (deq m n (iset a b))
+    -> pseq G (deq m n a).
+Proof.
+intros G a b m n.
+revert G.
+refine (seq_pseq 0 1 [] _ _ _); cbn.
+intros G Hseq.
+rewrite -> seq_deq in Hseq |- *.
+intros i s s' Hs.
+so (Hseq i s s' Hs) as (R & Hl & Hr & Hm & Hn & Hmn); clear Hseq.
+simpsubin Hl.
+simpsubin Hr.
+invert (basic_value_inv _#6 value_iset Hl).
+intros A B Ha Hb Heq1.
+invert (basic_value_inv _#6 value_iset Hr).
+intros A' B' Ha' Hb' Heq2.
+so (eqtrans Heq1 (eqsymm Heq2)) as Heq.
+clear Heq2.
+subst R.
+so (iuiset_inj _#5 Heq) as Heq'.
+injectionT Heq'.
+intros <-.
 exists A.
 do2 4 split; auto.
   {
@@ -658,6 +902,160 @@ do2 4 split; auto.
 Qed.
 
 
+Lemma sound_iset_elim2 :
+  forall G a b m J,
+    pseq G (deq m m (iset a b))
+    -> pseq (hyp_tm (subst1 m b) :: G) (substj sh1 J)
+    -> pseq G J.
+Proof.
+intros G a b m J.
+revert G.
+refine (seq_pseq 0 2 [] _ [_] _ _ _); cbn.
+intros G Hseqm Hseqnp.
+destruct J as [n p c].
+simpsubin Hseqnp.
+rewrite -> seq_deq in Hseqm, Hseqnp |- *.
+assert (forall i s s',
+          pwctx i s s' G
+          -> pwctx i (dot (subst s m) s) (dot (subst s' m) s') (hyp_tm a :: G)) as Hsm.
+  {
+  intros i s s' Hs.
+  apply pwctx_cons_tm_seq; auto.
+    {
+    so (Hseqm _#3 Hs) as (R & Hl & Hr & Hm & _).
+    simpsubin Hl.
+    simpsubin Hr.
+    invert (basic_value_inv _#6 value_iset Hl).
+    intros A B Hal _ Heq1.
+    invert (basic_value_inv _#6 value_iset Hr).
+    intros A' B' Har _ Heq2.
+    so (eqtrans Heq1 (eqsymm Heq2)) as Heq.
+    clear Heq2.
+    subst R.
+    so (iuiset_inj _#5 Heq) as Heq'.
+    injectionT Heq'.
+    intros <-.
+    cbn in Hm.
+    decompose Hm.
+    intros _ _ Hm' _.
+    apply (seqhyp_tm _#5 A); auto.
+    }
+
+    {
+    intros j u u' Hu.
+    so (Hseqm _#3 Hu) as (R & Hl & Hr & Hm & _).
+    simpsubin Hl.
+    simpsubin Hr.
+    invert (basic_value_inv _#6 value_iset Hl).
+    intros A B Hal _ Heq1.
+    invert (basic_value_inv _#6 value_iset Hr).
+    intros A' B' Har _ Heq2.
+    so (eqtrans Heq1 (eqsymm Heq2)) as Heq.
+    clear Heq2.
+    so (iuiset_inj _#5 Heq) as Heq'.
+    injectionT Heq'.
+    intros <-.
+    eauto.
+    }
+  }
+intros i s s' Hs.
+so (Hseqm _#3 Hs) as (R & Hl & Hr & Hm & _).
+simpsubin Hl.
+simpsubin Hr.
+invert (basic_value_inv _#6 value_iset Hl); clear Hl.
+intros A B Hal Hbl Heq1.
+invert (basic_value_inv _#6 value_iset Hr); clear Hr.
+intros A' B' Har Hbr Heq2.
+so (eqtrans Heq1 (eqsymm Heq2)) as Heq.
+clear Heq2.
+subst R.
+so (iuiset_inj _#5 Heq) as Heq'.
+injectionT Heq'.
+intros <-.
+injectionT Heq'.
+intros <-.
+clear Heq.
+cbn in Hm.
+decompose Hm.
+intros q r Hm Hqr.
+assert (pwctx i (dot q s) (dot r s') (hyp_tm (subst1 m b) :: G)) as Hsqr.
+  {
+  apply pwctx_cons_tm_seq; auto.
+    {
+    simpsub.
+    apply (seqhyp_tm _#5 (pi1 B (urelspinj _#4 Hm))); auto.
+      {
+      invert Hbl.
+      intros _ _ Hact.
+      so (Hact _#3 (le_refl _) Hm) as H.
+      simpsubin H.
+      exact H.
+      }
+
+      {
+      invert Hbr.
+      intros _ _ Hact.
+      so (Hact _#3 (le_refl _) Hm) as H.
+      simpsubin H.
+      exact H.
+      }
+    }
+    
+    {
+    clear i s s' A B q r Hs Hal Hbl Har Hbr Hm Hqr.
+    intros i s s' Hs.
+    so (Hseqm _#3 Hs) as (R & Hl & Hr & Hm & _).
+    simpsubin Hl.
+    simpsubin Hr.
+    invert (basic_value_inv _#6 value_iset Hl).
+    intros A B Hal Hbl Heq1.
+    invert (basic_value_inv _#6 value_iset Hr).
+    intros A' B' Har Hbr Heq2.
+    so (eqtrans Heq1 (eqsymm Heq2)) as Heq.
+    clear Heq2.
+    so (iuiset_inj _#5 Heq) as Heq'.
+    injectionT Heq'.
+    intros <-.
+    injectionT Heq'.
+    intros <-.
+    subst R.
+    clear Heq.
+    cbn in Hm.
+    decompose Hm.
+    intros _ _ Hm _.
+    exists toppg.
+    exists (pi1 B (urelspinj (den A) i (subst s m) (subst s' m) Hm)).
+    split.
+      {
+      invert Hbl.
+      intros _ _ Hact.
+      so (Hact _ _ _ (le_refl _) Hm) as H.
+      simpsubin H.
+      simpsub.
+      exact H.
+      }
+
+      {
+      invert Hbr.
+      intros _ _ Hact.
+      so (Hact _ _ _ (le_refl _) Hm) as H.
+      simpsubin H.
+      simpsub.
+      exact H.
+      }
+    }
+  }
+so (Hseqnp _#3 Hsqr) as (C & Hcl & Hcr & Hn & Hp & Hnp).
+simpsubin Hcl.
+simpsubin Hcr.
+simpsubin Hn.
+simpsubin Hp.
+simpsubin Hnp.
+exists C.
+do2 4 split; auto.
+Qed.
+
+
 Lemma interp_set_invert :
   forall pg s s' i a a' b b' R,
     interp pg s i (set a b) R
@@ -674,6 +1072,28 @@ intros A' B' Hal' _ Heq2.
 so (eqtrans Heq1 (eqsymm Heq2)) as Heq.
 clear Heq1 Heq2.
 so (iuset_inj _#5 Heq); subst A'.
+eauto.
+Qed.
+
+
+Lemma interp_iset_invert1 :
+  forall pg s s' i a a' b b' R,
+    interp pg s i (iset a b) R
+    -> interp pg s' i (iset a' b') R
+    -> exists A,
+         interp pg s i a A
+         /\ interp pg s' i a' A.
+Proof.
+intros pg s s' i a a' b b' R Hl Hr.
+invert (basic_value_inv _#6 value_iset Hl).
+intros A B Hal _ Heq1.
+invert (basic_value_inv _#6 value_iset Hr).
+intros A' B' Hal' _ Heq2.
+so (eqtrans Heq1 (eqsymm Heq2)) as Heq.
+clear Heq1 Heq2.
+so (iuiset_inj _#5 Heq) as Heq'.
+injectionT Heq'.
+intros <-.
 eauto.
 Qed.
 
@@ -1029,6 +1449,532 @@ do2 4 split.
 Qed.
 
 
+Lemma sound_iset_hyp_weaken :
+  forall G1 G2 a b J,
+    pseq (G2 ++ hyp_tm b :: hyp_tm a :: G1) J
+    -> pseq (G2 ++ hyp_tm b :: hyp_tm (iset a b) :: G1) J.
+Proof.
+intros G1 G2 a b J.
+revert G1.
+refine (seq_pseq_hyp 0 1 _ [_; _] _ _ [_; _] _ _); cbn.
+intros G Hseq HclJ.
+replace J with (substj (under (length G2) id) J) in Hseq by (simpsub; reflexivity).
+replace G2 with (substctx id G2) in Hseq by (simpsub; reflexivity).
+eapply (subsume_seq _ _ (under (length G2) id)); eauto.
+rewrite -> length_substctx.
+apply subsume_under.
+do2 2 split.
+  {
+  intros j.
+  split.
+    {
+    intros Hj.
+    simpsub.
+    apply hygiene_var.
+    rewrite -> ctxpred_length in Hj |- *.
+    cbn in Hj |- *.
+    omega.
+    }
+
+    {
+    intros Hj.
+    simpsub.
+    simpsubin Hj.
+    invertc Hj.
+    intro Hj.
+    rewrite -> ctxpred_length in Hj |- *.
+    cbn in Hj |- *.
+    omega.
+    }
+  }
+
+  {
+  intros j.
+  split.
+    {
+    intros Hj.
+    simpsub.
+    apply hygiene_var.
+    rewrite -> ctxpred_length in Hj |- *.
+    cbn in Hj |- *.
+    omega.
+    }
+
+    {
+    intros Hj.
+    simpsub.
+    simpsubin Hj.
+    invertc Hj.
+    intro Hj.
+    rewrite -> ctxpred_length in Hj |- *.
+    cbn in Hj |- *.
+    omega.
+    }
+  }
+intros i ss ss' Hss.
+invertc Hss.
+intros p q ss2 ss2' Hss Hpq Hleft2 Hright2 <- <-.
+invertc Hss.
+intros m n s s' Hs Hmn Hleft1 Hright1 <- <-.
+simpsubin Hmn.
+invertc Hmn.
+intros R Hsetl Hsetr Hmn.
+invertc Hpq.
+intros Bm Hbml Hbnr Hpq.
+invert (basic_value_inv _#6 value_iset Hsetl).
+intros A B Hal Hbl Heq1.
+invert (basic_value_inv _#6 value_iset Hsetr).
+intros A' B' Har Hbr Heq2.
+so (eqtrans Heq1 (eqsymm Heq2)) as Heq.
+clear Heq2.
+subst R.
+so (iuiset_inj _#5 Heq) as Heq'.
+injectionT Heq'.
+intros <-.
+so Hmn as Hmnset.
+cbn in Hmn.
+decompose Hmn.
+intros _ _ Hmn _.
+invert Hbl.
+intros _ _ Hact.
+so (Hact _ _ _ (le_refl _) Hmn) as H; clear Hact.
+simpsubin H.
+so (basic_fun _#7 Hbml H); subst Bm; clear H.
+do2 4 split.
+  {
+  simpsub.
+  apply pwctx_cons_tm.
+    {
+    apply pwctx_cons_tm; auto.
+      {
+      eapply seqhyp_tm; eauto.
+      }
+
+      {
+      intros j u Hj Hu.
+      exploit (Hleft1 j false u) as H; auto using smaller_le, pwctx_impl_seqctx.
+      rewrite -> qpromote_hyp_tm in H.
+      simpsubin H.
+      invertc H.
+      intros R Hsetr' Hsetu.
+      so (interp_iset_invert1 _#9 Hsetr' Hsetu) as (A' & Har' & Hau).
+      eapply relhyp_tm; eauto.
+      }
+
+      {
+      intros j u Hj Hu.
+      exploit (Hright1 j false u) as H; auto using smaller_le, pwctx_impl_seqctx.
+      rewrite -> qpromote_hyp_tm in H.
+      simpsubin H.
+      invertc H.
+      intros R Hsetu Hsetl'.
+      so (interp_iset_invert1 _#9 Hsetu Hsetl') as (A' & Har' & Hau).
+      eapply relhyp_tm; eauto.
+      }
+    }
+
+    {
+    eapply seqhyp_tm; eauto.
+    }
+
+    {
+    intros j uu Hj Huu.
+    exploit (Hleft2 j false uu) as H; auto using smaller_le, pwctx_impl_seqctx.
+    rewrite -> qpromote_cons.
+    cbn.
+    invertc Huu.
+    intros n' u Hu Hmn' _ _ <-.
+    apply seqctx_cons; auto using pwctx_impl_seqctx.
+    simpsub.
+    simpsubin Hmn'.
+    invertc Hmn'.
+    intros A' Hal' Hau Hmn'.
+    so (basic_fun _#7 (basic_downward _#7 Hj Hal) Hal'); subst A'; clear Hal'.
+    apply (seqhyp_tm _#5 (iutruncate (S j) (iuiset _ A B))).
+      {
+      eapply basic_downward; eauto.
+      }
+
+      {
+      exploit (Hleft1 j false u) as H; auto using smaller_le, pwctx_impl_seqctx.
+      rewrite -> qpromote_hyp_tm in H.
+      simpsubin H.
+      invertc H.
+      intros R Hsetr' Hsetu.
+      so (basic_fun _#7 (basic_downward _#7 Hj Hsetr) Hsetr'); subst R.
+      exact Hsetu.
+      }
+    
+      {
+      cbn.
+      split; [omega |].
+      destruct Hmn' as (_ & Hmn').
+      exists p, q, Hmn'.
+      refine (rel_from_dist _#6 _ (urel_downward_leq _#6 Hj Hpq)).
+      apply den_nonexpansive.
+      apply (pi2 B).
+      apply urelspinj_dist_diff; auto.
+      }
+    }
+
+    {
+    intros j uu Hj Huu.
+    exploit (Hright2 j false uu) as H; auto using smaller_le, pwctx_impl_seqctx.
+    rewrite -> qpromote_cons.
+    cbn.
+    invertc Huu.
+    intros m' u Hu Hmn' _ _ <-.
+    apply seqctx_cons; auto using pwctx_impl_seqctx.
+    simpsub.
+    simpsubin Hmn'.
+    invertc Hmn'.
+    intros A' Hau Har' Hmn'.
+    so (basic_fun _#7 (basic_downward _#7 Hj Har) Har'); subst A'; clear Har'.
+    apply (seqhyp_tm _#5 (iutruncate (S j) (iuiset _ A B))).
+    2:{
+      eapply basic_downward; eauto.
+      }
+
+      {
+      exploit (Hright1 j false u) as H; auto using smaller_le, pwctx_impl_seqctx.
+      rewrite -> qpromote_hyp_tm in H.
+      simpsubin H.
+      invertc H.
+      intros R Hsetl' Hsetu.
+      so (basic_fun _#7 (basic_downward _#7 Hj Hsetl) Hsetl'); subst R.
+      exact Hsetu.
+      }
+    
+      {
+      cbn.
+      split; [omega |].
+      destruct Hmn' as (_ & Hmn').
+      exists p, q, Hmn'.
+      refine (rel_from_dist _#6 _ (urel_downward_leq _#6 Hj Hpq)).
+      apply den_nonexpansive.
+      apply (pi2 B).
+      apply urelspinj_dist_diff; auto.
+      eapply urel_downward_leq; eauto.
+      }
+    }
+  }
+
+  {
+  simpsub.
+  apply equivsub_refl.
+  }
+
+  {
+  simpsub.
+  apply equivsub_refl.
+  }
+
+  {
+  intros j d uu Hsmall Huu.
+  so (smaller_impl_le _#3 Hsmall) as Hj.
+  simpsubin Huu.
+  simpsub.
+  rewrite -> !qpromote_cons in Huu |- *.
+  rewrite -> !qpromote_hyp_tm in Huu |- *.
+  invertc Huu.
+  intros q' uu2 Huu Hpq' <-.
+  invertc Huu.
+  intros n' u Hu Hmn' <-.
+  apply seqctx_cons.
+    {
+    apply seqctx_cons; auto.
+    simpsub.
+    apply (seqhyp_tm _#5 (iutruncate (S j) (iuiset stop A B))).
+      {
+      apply (basic_downward _#3 i); auto.
+      }
+
+      {
+      exploit (Hleft1 j d u) as H; auto.
+      rewrite -> qpromote_hyp_tm in H.
+      simpsubin H.
+      simpsub.
+      invertc H.
+      intros R Hsetr' Hsetu.
+      so (basic_fun _#7 (basic_downward _#7 Hj Hsetr) Hsetr'); subst R.
+      auto.
+      }
+
+      {
+      split; auto.
+      cbn.
+      simpsubin Hmn'.
+      invertc Hmn'.
+      intros R Hal' _ Hmn'.
+      so (basic_fun _#7 (basic_downward _#7 Hj Hal) Hal'); subst R.
+      destruct Hmn' as (_ & Hmn').
+      exists p, q, Hmn'.
+      refine (rel_from_dist _#6 _ (urel_downward_leq _#6 Hj Hpq)).
+      apply den_nonexpansive.
+      apply (pi2 B).
+      apply urelspinj_dist_diff; auto.
+      }
+    }
+
+    {
+    simpsub.
+    invertc Hmn'.
+    intros R Hal' _ Hmn'.
+    so (basic_fun _#7 (basic_downward _#7 Hj Hal) Hal'); subst R.
+    destruct Hmn' as (_ & Hmn').
+    invert Hbl.
+    intros _ _ Hact.
+    so (Hact _#3 Hj Hmn') as Hmblj; clear Hact.
+    simpsubin Hmblj.
+    simpsubin Hpq'.
+    invertc Hpq'.
+    intros R Hmblj' Hmbu Hpq'.
+    so (basic_fun _#7 Hmblj Hmblj'); subst R.
+    apply (seqhyp_tm _#5 (pi1 B (urelspinj _#4 Hmn'))); auto.
+    }
+  }
+
+  {
+  intros j d uu Hsmall Huu.
+  so (smaller_impl_le _#3 Hsmall) as Hj.
+  simpsubin Huu.
+  simpsub.
+  rewrite -> !qpromote_cons in Huu |- *.
+  rewrite -> !qpromote_hyp_tm in Huu |- *.
+  invertc Huu.
+  intros p' uu2 Huu Hpq' <-.
+  invertc Huu.
+  intros m' u Hu Hmn' <-.
+  apply seqctx_cons.
+    {
+    apply seqctx_cons; auto.
+    simpsub.
+    apply (seqhyp_tm _#5 (iutruncate (S j) (iuiset stop A B))).
+      {
+      exploit (Hright1 j d u) as H; auto.
+      rewrite -> qpromote_hyp_tm in H.
+      simpsubin H.
+      simpsub.
+      invertc H.
+      intros R Hsetl' Hsetu.
+      so (basic_fun _#7 (basic_downward _#7 Hj Hsetl) Hsetl'); subst R.
+      auto.
+      }
+
+      {
+      apply (basic_downward _#3 i); auto.
+      }
+
+      {
+      split; auto.
+      cbn.
+      simpsubin Hmn'.
+      invertc Hmn'.
+      intros R _ Har' Hmn'.
+      so (basic_fun _#7 (basic_downward _#7 Hj Har) Har'); subst R.
+      destruct Hmn' as (_ & Hmn').
+      exists p, q, Hmn'.
+      refine (rel_from_dist _#6 _ (urel_downward_leq _#6 Hj Hpq)).
+      apply den_nonexpansive.
+      apply (pi2 B).
+      apply urelspinj_dist_diff; auto.
+      eapply urel_downward_leq; eauto.
+      }
+    }
+
+    {
+    simpsub.
+    invertc Hmn'.
+    intros R _ Har' Hmn'.
+    so (basic_fun _#7 (basic_downward _#7 Hj Har) Har'); subst R.
+    destruct Hmn' as (_ & Hmn').
+    invert Hbr.
+    intros _ _ Hact.
+    so (Hact _#3 Hj Hmn') as Hmblj; clear Hact.
+    simpsubin Hmblj.
+    simpsubin Hpq'.
+    invertc Hpq'.
+    intros R Hmbu Hmblj' Hpq'.
+    so (basic_fun _#7 Hmblj Hmblj'); subst R.
+    apply (seqhyp_tm _#5 (pi1 B' (urelspinj _#4 Hmn'))); auto.
+    }
+  }
+Qed.
+
+
+Lemma sound_set_formation_invert :
+  forall G a a' b b',
+    pseq G (deqtype (set a b) (set a' b'))
+    -> pseq G (deqtype a a').
+Proof.
+intros G a b c d.
+revert G.
+refine (seq_pseq 0 1 [] _ _ _).
+cbn.
+intros G Hseq.
+rewrite -> seq_eqtype in Hseq |- *.
+intros i s s' Hs.
+so (Hseq _ _ _ Hs) as (R & Hacl & Hacr & Hbdl & Hbdr).
+simpsubin Hacl.
+invert (basic_value_inv _#6 value_set Hacl).
+intros A B1 Hal _ Heq.
+simpsubin Hacr.
+invert (basic_value_inv _#6 value_set Hacr).
+intros A' B2 Har _ Heq'.
+so (eqtrans Heq (eqsymm Heq')) as H.
+so (iuset_inj _#5 H); subst A'.
+clear H Heq'.
+simpsubin Hbdl.
+invert (basic_value_inv _#6 value_set Hbdl).
+intros A' B3 Hbl _ Heq'.
+so (eqtrans Heq (eqsymm Heq')) as H.
+so (iuset_inj _#5 H); subst A'.
+clear H Heq'.
+simpsubin Hbdr.
+invert (basic_value_inv _#6 value_set Hbdr).
+intros A' B4 Hbr _ Heq'.
+so (eqtrans Heq (eqsymm Heq')) as H.
+so (iuset_inj _#5 H); subst A'.
+clear H Heq' Heq.
+exists A.
+auto.
+Qed.
+
+
+Lemma sound_iset_formation_invert1 :
+  forall G a a' b b',
+    pseq G (deqtype (iset a b) (iset a' b'))
+    -> pseq G (deqtype a a').
+Proof.
+intros G a b c d.
+revert G.
+refine (seq_pseq 0 1 [] _ _ _).
+cbn.
+intros G Hseq.
+rewrite -> seq_eqtype in Hseq |- *.
+intros i s s' Hs.
+so (Hseq _ _ _ Hs) as (R & Hacl & Hacr & Hbdl & Hbdr).
+simpsubin Hacl.
+invert (basic_value_inv _#6 value_iset Hacl).
+intros A B1 Hal _ Heq.
+simpsubin Hacr.
+invert (basic_value_inv _#6 value_iset Hacr).
+intros A' B2 Har _ Heq'.
+so (eqtrans Heq (eqsymm Heq')) as H.
+so (iuiset_inj _#5 H) as Heq''.
+injectionT Heq''.
+intros <-.
+clear H Heq' Heq''.
+simpsubin Hbdl.
+invert (basic_value_inv _#6 value_iset Hbdl).
+intros A' B3 Hbl _ Heq'.
+so (eqtrans Heq (eqsymm Heq')) as H.
+so (iuiset_inj _#5 H) as Heq''.
+injectionT Heq''.
+intros <-.
+clear H Heq' Heq''.
+simpsubin Hbdr.
+invert (basic_value_inv _#6 value_iset Hbdr).
+intros A' B4 Hbr _ Heq'.
+so (eqtrans Heq (eqsymm Heq')) as H.
+so (iuiset_inj _#5 H) as Heq''.
+injectionT Heq''.
+intros <-.
+clear H Heq' Heq Heq''.
+exists A.
+auto.
+Qed.
+
+
+Lemma sound_iset_formation_invert2 :
+  forall G a a' b b',
+    pseq G (deqtype (iset a b) (iset a' b'))
+    -> pseq (cons (hyp_tm a) G) (deqtype b b').
+Proof.
+intros G a b c d.
+revert G.
+refine (seq_pseq_hyp 4 [] a [] b [hyp_emp] c [hyp_emp] d 1 [] [] _ [] [_] _ _); cbn.
+intros G Hcla Hclb Hclc Hcld Hseq _.
+rewrite -> seq_eqtype in Hseq |- *.
+intros i ss ss' Hss.
+so (pwctx_cons_invert_simple _#5 Hss) as H; clear Hss.
+destruct H as (m & p & s & s' & Hs & Hmp & -> & ->).
+so (Hseq i s s' Hs) as (R & Hpil & Hpir & Hpil' & Hpir').
+simpsubin Hpil.
+simpsubin Hpir.
+simpsubin Hpil'.
+simpsubin Hpir'.
+invert (basic_value_inv _#6 value_iset Hpil).
+intros A B Hal Hcl Heqacl.
+invert (basic_value_inv _#6 value_iset Hpir).
+intros A' B' Har Hcr Heqacr.
+so (eqtrans Heqacl (eqsymm Heqacr)) as Heq.
+clear Heqacr.
+invert (basic_value_inv _#6 value_iset Hpil').
+intros A'' B'' Hbl Hdl Heqbdl.
+so (eqtrans Heqacl (eqsymm Heqbdl)) as Heq'.
+clear Heqbdl.
+invert (basic_value_inv _#6 value_iset Hpir').
+intros A''' B''' Hbr Hdr Heqbdr.
+so (eqtrans Heqacl (eqsymm Heqbdr)) as Heq''.
+clear Heqbdr.
+subst R.
+so (iuiset_inj _#5 Heq) as H.
+injectionT H.
+intros <-.
+injectionT H.
+intros <-.
+so (iuiset_inj _#5 Heq') as H.
+injectionT H.
+intros <-.
+injectionT H.
+intros <-.
+so (iuiset_inj _#5 Heq'') as H.
+injectionT H.
+intros <-.
+injectionT H.
+intros <-.
+clear Heq Heq' Heq''.
+invertc Hmp.
+intros A' Hal' _ Hmp.
+so (basic_fun _#7 (interp_increase _#6 (toppg_max _) Hal) Hal'); subst A'.
+exists (pi1 B (urelspinj (den A) i m p Hmp)).
+simpsub.
+do2 3 split.
+  {
+  invert Hcl.
+  intros _ _ Hact.
+  so (Hact _#3 (le_refl _) Hmp) as H.
+  simpsubin H.
+  exact H.
+  }
+
+  {
+  invert Hcr.
+  intros _ _ Hact.
+  so (Hact _#3 (le_refl _) Hmp) as H.
+  simpsubin H.
+  exact H.
+  }
+
+  {
+  invert Hdl.
+  intros _ _ Hact.
+  so (Hact _#3 (le_refl _) Hmp) as H.
+  simpsubin H.
+  exact H.
+  }
+
+  {
+  invert Hdr.
+  intros _ _ Hact.
+  so (Hact _#3 (le_refl _) Hmp) as H.
+  simpsubin H.
+  exact H.
+  }
+Qed.
+
+
 Lemma unit_urel_dist :
   forall i i' j,
     j <= i
@@ -1351,43 +2297,4 @@ split.
   apply urelspinj_dist_diff; auto.
   eapply urel_downward_leq; eauto.
   }
-Qed.
-
-
-Lemma sound_set_formation_invert :
-  forall G a a' b b',
-    pseq G (deqtype (set a b) (set a' b'))
-    -> pseq G (deqtype a a').
-Proof.
-intros G a b c d.
-revert G.
-refine (seq_pseq 0 1 [] _ _ _).
-cbn.
-intros G Hseq.
-rewrite -> seq_eqtype in Hseq |- *.
-intros i s s' Hs.
-so (Hseq _ _ _ Hs) as (R & Hacl & Hacr & Hbdl & Hbdr).
-simpsubin Hacl.
-invert (basic_value_inv _#6 value_set Hacl).
-intros A B1 Hal _ Heq.
-simpsubin Hacr.
-invert (basic_value_inv _#6 value_set Hacr).
-intros A' B2 Har _ Heq'.
-so (eqtrans Heq (eqsymm Heq')) as H.
-so (iuset_inj _#5 H); subst A'.
-clear H Heq'.
-simpsubin Hbdl.
-invert (basic_value_inv _#6 value_set Hbdl).
-intros A' B3 Hbl _ Heq'.
-so (eqtrans Heq (eqsymm Heq')) as H.
-so (iuset_inj _#5 H); subst A'.
-clear H Heq'.
-simpsubin Hbdr.
-invert (basic_value_inv _#6 value_set Hbdr).
-intros A' B4 Hbr _ Heq'.
-so (eqtrans Heq (eqsymm Heq')) as H.
-so (iuset_inj _#5 H); subst A'.
-clear H Heq' Heq.
-exists A.
-auto.
 Qed.
