coq/ValidationSet.v
@@ -23,7 +23,7 @@ Require Import ValidationUtil.
 Require Import Defined.
 
 
-Hint Rewrite def_set def_squash : prepare.
+Hint Rewrite def_set def_iset def_squash : prepare.
 
 
 Lemma subst_squash :
@@ -51,11 +51,27 @@ eapply (tr_set_formation _#5 (var 0) (var 0)); eauto.
 Qed.
 
 
+Lemma isetForm_valid : isetForm_obligation.
+Proof.
+prepare.
+intros G a b ext1 ext0 Ha Hb.
+eapply (tr_iset_formation _#5); eauto.
+Qed.
+
+
 Lemma setEq_valid : setEq_obligation.
 Proof.
 prepare.
 intros G a b c d ext4 ext3 ext2 ext1 ext0 Hab Hc Hd Hcd Hdc.
 eapply tr_set_formation; eauto.
+Qed.
+
+
+Lemma isetEq_valid : isetEq_obligation.
+Proof.
+prepare.
+intros G a b c d ext1 ext0 Hab Hcd.
+eapply tr_iset_formation; eauto.
 Qed.
 
 
@@ -74,11 +90,27 @@ eapply (tr_set_formation_univ _#6 (var 0) (var 0)); eauto.
 Qed.
 
 
+Lemma isetFormUniv_valid : isetFormUniv_obligation.
+Proof.
+prepare.
+intros G a b i ext1 ext0 Ha Hb.
+eapply (tr_iset_formation_univ _#6); eauto.
+Qed.
+
+
 Lemma setEqUniv_valid : setEqUniv_obligation.
 Proof.
 prepare.
 intros G a b c d i ext4 ext3 ext2 ext1 ext0 Hab Hc Hd Hcd Hdc.
 eapply tr_set_formation_univ; eauto.
+Qed.
+
+
+Lemma isetEqUniv_valid : isetEqUniv_obligation.
+Proof.
+prepare.
+intros G a b c d i ext1 ext0 Hab Hcd.
+eapply tr_iset_formation_univ; eauto.
 Qed.
 
 
@@ -90,11 +122,27 @@ eapply tr_set_elim1; eauto.
 Qed.
 
 
+Lemma isetWeakenOf_valid : isetWeakenOf_obligation.
+Proof.
+prepare.
+intros G a b m ext0 H.
+eapply tr_iset_elim1; eauto.
+Qed.
+
+
 Lemma setWeakenEq_valid : setWeakenEq_obligation.
 Proof.
 prepare.
 intros G a b m n ext0 H.
 eapply tr_set_elim1; eauto.
+Qed.
+
+
+Lemma isetWeakenEq_valid : isetWeakenEq_obligation.
+Proof.
+prepare.
+intros G a b m n ext0 H.
+eapply tr_iset_elim1; eauto.
 Qed.
 
 
@@ -106,11 +154,27 @@ eapply tr_set_elim1; eauto.
 Qed.
 
 
+Lemma isetWeaken_valid : isetWeaken_obligation.
+Proof.
+prepare.
+intros G a b m H.
+eapply tr_iset_elim1; eauto.
+Qed.
+
+
 Lemma setIntroOf_valid : setIntroOf_obligation.
 Proof.
 prepare.
 intros G a b m ext2 ext1 ext0 Hb Hm Hmb.
 eapply tr_set_intro; eauto.
+Qed.
+
+
+Lemma isetIntroOf_valid : isetIntroOf_obligation.
+Proof.
+prepare.
+intros G a b m ext2 ext1 ext0 Hb Hm Hmb.
+eapply tr_iset_intro; eauto.
 Qed.
 
 
@@ -122,11 +186,27 @@ eapply tr_set_intro; eauto.
 Qed.
 
 
+Lemma isetIntroEq_valid : isetIntroEq_obligation.
+Proof.
+prepare.
+intros G a b m n ext2 ext1 ext0 Hb Hmn Hmb.
+eapply tr_iset_intro; eauto.
+Qed.
+
+
 Lemma setIntro_valid : setIntro_obligation.
 Proof.
 prepare.
 intros G a b m ext2 ext1 ext0 Hb Hm Hmb.
 eapply tr_set_intro; eauto.
+Qed.
+
+
+Lemma isetIntro_valid : isetIntro_obligation.
+Proof.
+prepare.
+intros G a b m ext2 ext1 ext0 Hb Hm Hmb.
+eapply tr_iset_intro; eauto.
 Qed.
 
 
@@ -264,6 +344,19 @@ auto.
 Qed.
 
 
+Lemma isetElim_valid : isetElim_obligation.
+Proof.
+prepare.
+intros G a b c m ext0 n Hhyg Hm Hn.
+eapply tr_iset_elim2; eauto.
+so (subst_into_absent_single _ 0 n triv Hhyg) as H.
+simpsubin H.
+simpsub.
+rewrite -> H.
+auto.
+Qed.
+
+
 Lemma tr_set_left :
   forall G1 G2 a b c m,
     hygiene (fun i => i <> length G2) m
@@ -383,11 +476,196 @@ apply (tr_set_elim2 _ (subst (sh (S k)) a) (subst (under 1 (sh (S k))) b) (var k
 Qed.
 
 
+Lemma tr_iset_left :
+  forall G1 G2 a b c m,
+    hygiene (fun i => i <> length G2) m
+    -> tr (substctx sh1 G2 ++ hyp_tm b :: hyp_tm a :: G1) (deq m m (subst (under (length G2) sh1) c))
+    -> tr (G2 ++ hyp_tm (iset a b) :: G1)
+         (deq
+            (subst (under (length G2) (dot triv id)) m)
+            (subst (under (length G2) (dot triv id)) m)
+            c).
+Proof.
+intros G1 G2 a b c m Hhyg Hm.
+set (k := length G2) in * |- *.
+apply (tr_iset_elim2 _ (subst (sh (S k)) a) (subst (under 1 (sh (S k))) b) (var k)).
+  {
+  eapply hypothesis.
+    {
+    apply (index_app_right _ G2 _ 0).
+    apply index_0.
+    }
+  simpsub.
+  auto.
+  }
+
+  {
+  simpsub.
+  replace (S k + 1) with (S (S k)) by omega.
+  simpsub.
+  apply (exchange_1_n _ G2 _ []).
+    {
+    simpsub.
+    rewrite -> project_unlift_ge; try omega.
+    replace (k - length G2) with 0 by omega.
+    fold k.
+    simpsub.
+    replace (k + 0) with k by omega.
+    rewrite <- compose_assoc.
+    rewrite -> compose_sh_unlift_ge; try omega.
+    simpsub.
+    replace (S k - k + k) with (S k) by omega.
+    auto.
+    }
+  cbn [length].
+  simpsub.
+  cbn [List.app].
+  rewrite -> project_unlift_ge; try omega.
+  replace (k - length G2) with 0 by omega.
+  rewrite -> compose_sh_unlift_ge; try omega.
+  fold k.
+  replace (S k - k) with 1 by omega.
+  rewrite -> subst_var0_sh1.
+  replace (dots 0 k (sh (S k))) with (@under obj k (sh 1)).
+  2:{
+    rewrite -> under_dots.
+    simpsub.
+    reflexivity.
+    }
+  rewrite <- compose_under.
+  simpsub.
+  so (subst_into_absent_single _ k m triv Hhyg) as H.
+  rewrite -> H.
+  apply tr_iset_hyp_weaken.
+  exact Hm.
+  }
+Qed.
+
+
+Lemma isetIntroOfSquash_valid : isetIntroOfSquash_obligation.
+Proof.
+prepare.
+intros G a b m ext2 ext1 ext0 Hb Hm Hmb.
+apply (tr_assert _ (squash (subst1 m b)) ext0).
+  {
+  simpsubin Hmb.
+  exact Hmb.
+  }
+replace (substj sh1 (deq m m (iset a b))) with (deq (subst (under 0 (dot triv id)) (subst (sh 2) m)) (subst (under 0 (dot triv id)) (subst (sh 2) m)) (subst sh1 (iset a b))).
+2:{
+  simpsub.
+  auto.
+  }
+apply (tr_set_left _ []).
+  {
+  cbn.
+  eapply hygiene_shift'.
+  apply (hygiene_weaken _ okay); auto using hygiene_okay.
+  intros j Hj.
+  omega.
+  }
+
+  {
+  simpsub.
+  eapply (weakening _ [_] []).
+    {
+    cbn [unlift length].
+    simpsub.
+    auto.
+    }
+
+    {
+    cbn [unlift length].
+    simpsub.
+    auto.
+    }
+  cbn [unlift length].
+  simpsub.
+  cbn [List.app].
+  apply (tr_generalize _ a m (deqtype b b)); auto.
+  }
+
+  {
+  simpsub.
+  cbn [List.app].
+  eapply (weakening _ [_] [_]).
+    {
+    cbn [unlift length].
+    simpsub.
+    auto.
+    }
+
+    {
+    cbn [unlift length].
+    simpsub.
+    auto.
+    }
+  cbn [unlift length].
+  simpsub.
+  cbn [List.app].
+  eapply (tr_iset_intro _#5 (var 0)).
+    {
+    eapply (weakening _ [_] []).
+      {
+      cbn [unlift length].
+      simpsub.
+      auto.
+      }
+  
+      {
+      cbn [unlift length].
+      simpsub.
+      auto.
+      }
+    cbn [unlift length].
+    simpsub.
+    cbn [List.app].
+    exact Hm.
+    }
+
+    {
+    simpsub.
+    eapply hypothesis; eauto using index_0.
+    simpsub.
+    auto.
+    }
+
+    {
+    eapply (weakening _ [_] [_]).
+      {
+      cbn [unlift length].
+      simpsub.
+      auto.
+      }
+  
+      {
+      cbn [unlift length].
+      simpsub.
+      auto.
+      }
+    cbn [unlift length].
+    simpsub.
+    cbn [List.app].
+    rewrite -> subst_var0_sh1.
+    exact Hb.
+    }
+  }
+Qed.
+
+
 Lemma setLeft_valid : setLeft_obligation.
 Proof.
 prepare.
 intros G1 G2 a b c ext0 m Hhyg Hb Hm.
 apply tr_set_left; auto.
+Qed.
+
+
+Lemma isetLeft_valid : isetLeft_obligation.
+Proof.
+prepare.
+intros G1 G2 a b c m Hhyg Hm.
+apply tr_iset_left; auto.
 Qed.
 
 
@@ -404,6 +682,30 @@ Proof.
 prepare.
 intros G a b ext0 H.
 eapply tr_set_formation_invert; eauto.
+Qed.
+
+
+Lemma isetFormInv1_valid : isetFormInv1_obligation.
+Proof.
+prepare.
+intros G a b ext0 H.
+eapply tr_iset_formation_invert1; eauto.
+Qed.
+
+
+Lemma isetFormInv2_valid : isetFormInv2_obligation.
+Proof.
+prepare.
+intros G a b m ext0 ext1 Hsig Hm.
+simpsub.
+cut (tr (hyp_tm a :: G) (deqtype b b)).
+  {
+  intro Hb.
+  so (tr_generalize _#4 Hm Hb) as H.
+  simpsubin H.
+  exact H.
+  }
+eapply tr_iset_formation_invert2; eauto.
 Qed.
 
 
@@ -454,6 +756,53 @@ apply tr_subtype_intro.
 
     {
     eapply tr_set_elim1.
+    eapply hypothesis; eauto using index_0.
+    simpsub.
+    reflexivity.
+    }
+  }
+Qed.
+
+
+Lemma isetSubElim_valid : isetSubElim_obligation.
+Proof.
+prepare.
+intros G a c b ext1 ext0 Hac Hb.
+apply tr_subtype_intro.
+  {
+  apply tr_iset_formation; eauto.
+    {
+    eapply tr_subtype_istype1; eauto.
+    }
+  }
+
+  {
+  eapply tr_subtype_istype2; eauto.
+  }
+
+  {
+  apply (tr_subtype_elim _ (subst sh1 a)).
+    {
+    eapply (weakening _ [_] []).
+      {
+      cbn [length unlift].
+      simpsub.
+      auto.
+      }
+
+      {
+      cbn [length unlift].
+      simpsub.
+      auto.
+      }
+    cbn [length unlift].
+    simpsub.
+    cbn [List.app].
+    exact Hac.
+    }
+
+    {
+    eapply tr_iset_elim1.
     eapply hypothesis; eauto using index_0.
     simpsub.
     reflexivity.
